More proofs

Examples/Paxos/PaxosAcceptor.v
@@ -96,19 +96,29 @@ Next Obligation.
 Qed.
 
 Program Definition read_state:
-  {(e: nat) (rs: RoleState)}, DHT [a, W]
-  (fun i => loc i = st :-> (e, rs), 
-   fun r m => loc m = st :-> (e, rs) /\
+  {(s: StateT)}, DHT [a, W]
+  (fun i => loc i = st :-> s, 
+   fun r m => loc m = st :-> s /\
               exists (pf : coh (getS m)), r = (getSt a pf).2) :=
   Do (act (@skip_action_wrapper W a l paxos (prEq paxos) _
                                 (fun s pf => (getSt a pf).2))).
 Next Obligation.
-  admit.
-Admitted.
+  apply: ghC.
+  move => s st s_is_st s_in_coh_w.
+  apply: act_rule => j R.
+  split => [|r k m].
+    by case: (rely_coh R).
+  case=>/=H1[Cj]Z.
+  subst j=>->R'.
+  split; first by rewrite (rely_loc' l R') (rely_loc' _ R).
+  case: (rely_coh R')=>_; case=>_ _ _ _/(_ l)=>/= pf; rewrite prEq in pf.
+  exists pf; move: (rely_loc' l R') =>/sym E'.
+  suff X: getSt a (Actions.safe_local (prEq paxos) H1) = getSt a pf by rewrite X.
+  by apply: (getStE pf _ E'). 
+Qed.
 
 (* Step 1: Receive prepare req *)
 
-(* TODO: Check ending condition *)
 (* Ending condition *)
 Definition r_prepare_req_cond (res : option proposal) := res == None.
 
@@ -119,18 +129,6 @@ Definition r_prepare_req_inv (e : nat) (pinit: proposal): cont (option proposal)
     if res is Some psal
     then loc i = st :-> (e, APromised psal)
     else loc i = st :-> (e, AInit).
-
-  (* (fun i => loc i = st :-> (e, AInit), *)
-  (*  fun res m => exists psal, res = Some psal /\ loc m = st :-> (e, APromised psal)) *)
-  (* := *)
-  (* Do _ (@while a W _ _ r_prepare_req_cond (r_prepare_req_inv e) _ *)
-  (*       (fun _ => Do _ ( *)
-  (*          r <-- tryrecv_prepare_req; *)
-  (*          match r with *)
-  (*          | Some (from, tg, body) => ret _ _ (Some body) *)
-  (*          | None => ret _ _ None *)
-  (*          end               *)
-  (*       )) None). *)
 
 (* Loops until it receives a prepare req *)
 Program Definition receive_prepare_req_loop (e : nat):
@@ -195,10 +193,12 @@ Definition read_promised_value (rs: RoleState) :=
 
 (* Step 2: Respond promise or nack to the proposer *)
 Program Definition resp_to_prepare_req (e: nat) (prepare_no: nat):
-  {(pinit pfinal: proposal)}, DHT [a, W]
-   (fun i => loc i = st :-> (e, APromised pinit) \/ loc i = st :-> (e, AInit),
-    fun (_ : seq nat) m => loc m = st :-> (e, APromised pinit) \/
-        loc m = st :-> (e, APromised pfinal))
+  {(pif: (proposal * proposal))}, DHT [a, W]
+   (fun i => loc i = st :-> (e, APromised pif.1) \/ loc i = st :-> (e, AInit),
+    fun (_ : seq nat) m =>
+      if head 0 pif.2 > head 0 pif.1
+      then loc m = st :-> (e, APromised pif.2)
+      else loc m = st :-> (e, APromised pif.1))
   := Do (rs <-- read_state;
          let: promised := read_promised_number rs in
          let: value := read_promised_value rs in  
@@ -206,7 +206,29 @@ Program Definition resp_to_prepare_req (e: nat) (prepare_no: nat):
          then send_promise_resp [:: promised; value] prepare_no
          else send_nack_resp [:: 0; 0] prepare_no).
 Next Obligation.
-  admit.
+  apply:ghC=>i [pinit pfinal]E1 C1.
+  have Pre: forall i2 proposer_id, network_rely W a i i2 ->
+          Actions.send_act_safe W (p:=paxos) a l
+          (* can't call read_state to find which transition to send *)
+          (if prepare_no > 0
+           then (
+               send_promise_resp_trans proposers acceptors
+           )
+           else (
+               send_nack_resp_trans proposers acceptors
+          )) [:: e] proposer_id i2.
+  - move=>i2 pid R1.
+    split; first by case: (rely_coh R1).
+    case: (proj2 (rely_coh R1))=>_ _ _ _/(_ l); rewrite (prEq paxos)=>C.
+    admit.
+    
+    (* Need inE to work *)
+    (* + rewrite /Actions.can_send /nodes inE/= mem_cat Hpin orbC. *)
+    (* by rewrite -(cohD (proj2 (rely_coh R1)))/ddom gen_domPt inE/= eqxx. *)
+    admit.
+    by rewrite /Actions.filter_hooks um_filt0=>???/sym/find_some; rewrite dom0 inE.
+
+    admit.
 Admitted.
 
 (* TODO: Check ending condition *)
@@ -215,21 +237,25 @@ Definition r_acc_req_cond (res : option proposal) := res == None.
 
 (* ??  Do I need to check the higher proposal number according to the state? *)
 (* Invariant relates the argument and the shape of the state *)
-Definition r_acc_req_inv (e : nat) (psal: proposal) : cont (option proposal) :=
+Definition r_acc_req_inv (e : nat) (promised: bool) (psal: proposal): cont (option proposal) :=
   fun res i =>
     if res is Some psal
     then loc i = st :-> (e, AAccepted psal)
-    else loc i = st :-> (e, AInit).
+    else if promised
+         then loc i = st :-> (e, APromised psal)
+         else loc i = st :-> (e, AInit).
 
 (* Loops until it receives a accept req *)
-Program Definition receive_acc_req_loop (e : nat):
+Program Definition receive_acc_req_loop (e : nat) (promised: bool):
   {(pinit: proposal)}, DHT [a, W]
-  (fun i => loc i = st :-> (e, AInit) \/ loc i = st :-> (e, APromised),
+   (fun i => if promised
+             then loc i = st :-> (e, APromised pinit)
+             else loc i = st :-> (e, AInit),
   fun res m => exists psal, res = Some psal /\ (
     loc m = st :-> (e, APromised psal) \/
     loc m = st :-> (e, AAccepted psal)
   )) :=
-  Do _ (@while a W _ _ r_acc_req_cond (r_acc_req_inv e) _
+  Do _ (@while a W _ _ r_acc_req_cond (r_acc_req_inv e promised) _
         (fun _ => Do _ (
            r <-- tryrecv_accept_req;
            match r with
@@ -258,26 +284,33 @@ Next Obligation.
   have D: rt = receive_accept_req_trans _ _.
   -  move: Hin G. clear E1.
      case => //. move => ->.
+     admit.
   admit.
+  apply: ret_rule=>//i5 R4.
+  - rewrite /r_acc_req_inv (rely_loc' _ R4) (rely_loc' _ R) locE//=.
+    rewrite -(rely_loc' _ R1) in E1.
+    rewrite D.
+    rewrite/step_recv/=.
+    rewrite /r_step.
+    rewrite /step_recv/=.
 Admitted.
 Next Obligation.
   apply: ghC=>i1 psal E1 C1/=.
-  apply: (gh_ex (g := psal)). apply: call_rule => //[r|r i2 [H1]H2 C2].
-  admit.
+  apply: (gh_ex (g := psal)); apply: call_rule => //r i2 [H1]H2 C2.
   rewrite /r_acc_req_cond/r_acc_req_inv in H1 H2; case: r H1 H2=>//b _ i2_AA.
   exists b.
   by split => //; right.
-Admitted.
+Qed.
 
 (* Using resp_to_prepare_req 0 as a 'do nothing' transition for now.
 As 0 will never be > 0 so the acceptor won't send a promise *)
 Program Definition acceptor_round:
-  {(e: nat) (psal: proposal)}, DHT [a, W] 
-  (fun i => loc i = st :-> (e, AInit) \/ loc i = st :-> (e, APromised psal),
+  {(ep: nat * proposal)}, DHT [a, W] 
+  (fun i => loc i = st :-> (ep.1, AInit),
    fun (_: unit) m => (
-     loc m = st :-> (e, AInit) \/
-     loc m = st :-> (e, APromised psal) \/
-     loc m = st :-> (e, AAccepted psal)
+     loc m = st :-> (ep.1, AInit) \/
+     loc m = st :-> (ep.1, APromised ep.2) \/
+     loc m = st :-> (ep.1, AAccepted ep.2)
   )) :=
     Do _ (e <-- read_round;
           msg <-- receive_prepare_req_loop e;
@@ -287,11 +320,15 @@ Program Definition acceptor_round:
              resp_to_prepare_req e p_no
            | _  => resp_to_prepare_req e 6
           end);;
-         receive_acc_req_loop e;;
+         rs <-- read_state;
+         (match rs with
+         | APromised _ => receive_acc_req_loop e true
+         | _  => receive_acc_req_loop e false
+         end);;
          ret _ _ tt).
-         (** ?? I think don't need to respond to accept request as the step_recv
-          function in the protocol file handles updating state? *)
 Next Obligation.
+  (* apply:ghC=>i1[e lg]/=E1 C1;  apply: step. *)
+  (* apply: (gh_ex (g:=(e, AInit))); apply: call_rule=>//e' i2 [E2][pf]->C2. *)
   admit.
 Admitted.
 
