Examples/Paxos/PaxosProposer.v
@@ -296,25 +296,27 @@ Qed.
 (*****************************************************)
 
 (* This is only ment to be run once for each proposer *)
-Program Definition proposer_round (psal: proposal):
-  {(e : nat)}, DHT [p, W]
+Program Definition proposer_round (p_init: proposal):
+  {(psal: proposal) (e : nat)}, DHT [p, W]
   (fun i => loc i = st :-> (e, PInit psal),
    fun res m => loc m = st :-> (e.+1, PAbort))
   :=
   Do (e <-- read_round;
-      send_prepare_req_loop e psal;;
+      send_prepare_req_loop e p_init;;
       recv_promises <-- receive_prepare_resp_loop e;
-      send_accept_reqs e (create_proposal_for_acc_req recv_promises psal)).
+      send_accept_reqs e (create_proposal_for_acc_req recv_promises p_init);;
+      ret _ _ true).
 Next Obligation.
-  move=>s0/=[e]E0; apply: step.
+  move=>s0/=[psal [e]] E0. apply: step.
   apply: (gh_ex (g := (e, PInit psal))).
   apply: call_rule=>//e' s1 [E1][pf]->C1.
   rewrite !(getStP_K _ E1)=>{e'}.
   apply: step; apply: (gh_ex (g := psal)).
   apply: call_rule=>//_ s2[_]/=E2 C2.
-  apply: step; apply: (gh_ex (g:=(psal))).
+  apply: step; apply: (gh_ex (g:=psal)).
   apply: call_rule=>//res s3/= [E3 H3] C3.
-  
+  apply: step; apply: (gh_ex (g:=e)); apply: (gh_ex (g:=d));
+  apply: (gh_ex (g:=lg)); apply: (gh_ex (g:=res)).
   admit.
 Admitted.
 
